\begin{frame}{Retour sur les équations produits}
    \section{Retour sur les équations produits}

    Résoudre :

    \begin{multicols}{2}
        \noindent$$(4x-28)(-3x-5)=0$$\vspace*{0.4\textheight}\columnbreak

        \noindent$$4x^2-49=0$$\vspace*{0.4\textheight}
    \end{multicols}
    \vfil
\end{frame}

% \begin{frame}{Retour sur les équations produits}
%     \section{Retour sur les équations produits}

%     Correction :

%     \begin{multicols}{2}
%         \begin{align*}
%             &(4x-28)(-3x-5)=0\\
%             \Rightarrow& 4x-28=0 \text{~ou~} -3x-5=0\\
%             \Rightarrow & 4x=28 \hspace*{1cm}\Rightarrow  -3x=5\\
%             \Rightarrow & x=7 \hspace*{1cm}\Rightarrow  x=\dfrac{-5}{3}\\
%             &\mathcal{S}=\left\{7;\dfrac{-5}{3}\right\}
%         \end{align*}
        

%         \begin{align*}
%             &4x^2-49=0\\
%             \Rightarrow & (2x)^2-7^2=0\\
%             \Rightarrow&(2x-7)(2x+7)=0\\
%             \Rightarrow&2x-7=0 &\text{~ou~} &2x+7=0\\
%             \Rightarrow&2x=7 &\Rightarrow 2x=-7&\\
%             \Rightarrow&x=\dfrac{7}{2} &\Rightarrow x=-\dfrac{7}{2}&\\
%             &\mathcal{S}=\left\{\dfrac{7}{2};-\dfrac{7}{2}\right\}
%         \end{align*}
%     \end{multicols}
%     \vfil
% \end{frame}