\begin{multicols}{3}
    \exo{Chercher}{OuParantheses1}\\
    $(5+3)\times 2-1=7$

    \exo{Chercher}{OuParantheses2}\\
    $5+3\times (2-1)=8$

    \exo{Chercher}{OuParantheses3}\\
    $(13+3): 4 +1=5$
\end{multicols}

\begin{multicols}{3}
    \exo{Calculer}{OuParantheses4}\\
    $4-(2+1)=1$

    \exo{Calculer}{OuParantheses5}\\
    $10-(7-3)+2=8$

    \exo{Calculer}{OuParantheses6}\\
    $10-((7-3)+2)=4$
\end{multicols}

\begin{multicols}{3}
    \exo{Calculer}{OuParantheses7}\\
    $4\times (3+2-1)=16$

    \exo{Calculer}{OuParantheses8}\\
    $(5+3)\times (4-2)=16$

    \exo{Calculer}{OuParantheses9}\\
    $12-(4\times 2+1)=3$
\end{multicols}

\begin{multicols}{3}
    \exo{Calculer}{OuParantheses10}\\
    $4\times (3+2)-1=19$

    \exo{Calculer}{OuParantheses11}\\
    $5+3\times (4-2)=11$

    \exo{Calculer}{OuParantheses12}\\
    $12-4\times (2+1)=0$
\end{multicols}