\consigne{EqProduitFacto1}{EqProduitFacto12} RÃ©soudre les equations produits suivantes

\begin{multicols}{2}
\exo{Raisonner}{EqProduitFacto1} 
$$(-7x-3)(-8x-10)+(-7x-3)(-2x+8)=0$$

\exo{Raisonner}{EqProduitFacto2} 
$$(-7x-5)(-4x-1)+(-7x-5)(-5x-8)=0$$

\exo{Raisonner}{EqProduitFacto3} 
$$( 9x-5)(-2x-6)+( 9x-5)(-5x-10)=0$$

\exo{Raisonner}{EqProduitFacto4} 
$$(-3x-1)( 2x-1)+(-3x-1)(-2x-4)=0$$

\exo{Raisonner}{EqProduitFacto5} 
$$( 10x-3)( 4x-1)-( 10x-3)( 9x+1)=0$$

\exo{Raisonner}{EqProduitFacto6} 
$$( 5x-1)(-7x-9)-( 5x-1)( 2x-6)=0$$

\exo{Raisonner}{EqProduitFacto7} 
$$(-8x-4)( 2x+10)-(-8x-4)( 6x+4)=0$$

\exo{Raisonner}{EqProduitFacto8} 
$$( 6x+6)(-5x-10)-( 6x+6)( 6x-3)=0$$

\exo{Raisonner}{EqProduitFacto9} 
$$(-10x-9)(-4x-10)=-(-10x-9)( 2x+3)$$

\exo{Raisonner}{EqProduitFacto10} 
$$( 1x-8)(-6x-7)=-( 1x-8)(-2x-4)$$

\exo{Raisonner}{EqProduitFacto11} 
$$( 6x-7)( 7x-7)= ( 6x-7)(-10x-3)$$

\exo{Raisonner}{EqProduitFacto12} 
$$( 8x-5)( 9x-3)= ( 8x-5)( 8x-2)$$

\end{multicols}