\begin{multicols}{2}
    \exo{Type Brevet}{Etape1}
    \begin{enumerate}
        \item On pose $A=(x-4)^2-x(x-10)$
        \item Développer et réduire $A$.
        \item Résoudre l'équation $A=16$.
    \end{enumerate}

    \exo{Type Brevet}{Etape2}
    \begin{enumerate}
        \item On pose $B=(x-2)^2-x(x-3)$
        \item Développer et réduire $B$.
        \item Résoudre l'équation $B=x+1$.
    \end{enumerate}

    \exo{Type Brevet}{Etape3}
    \begin{enumerate}
        \item On pose $C=(2x-4)^2+x(5x-16)$
        \item Développer et réduire $C$.
        \item Résoudre l'équation $C=20$.
    \end{enumerate}

    \exo{Type Brevet}{Etape4}
    \begin{enumerate}
        \item On pose $D=(7x-3)^2-5^2$
        \item Factoriser $D$.
        \item Résoudre l'équation $D=0$.
    \end{enumerate}
    \columnbreak

    \exo{Type Brevet}{Etape5}
    \begin{enumerate}
        \item On pose $E=(2x+3)^2+(x-5)(2x+3)$
        \item Factoriser $E$.
        \item Résoudre l'équation $E=0$.
    \end{enumerate}

    \exo{Type Brevet}{Etape6}
    \begin{enumerate}
        \item On pose $F=9x^2-25+(3x-5)(2x+15)$
        \item Factoriser $9x^2-25$ puis $F$.
        \item Résoudre l'équation $F=0$.
    \end{enumerate}

    \exo{Type Brevet}{Etape7}
    \begin{enumerate}
        \item On pose $G=(x-1)(2x+5)-(x-1)^2$
        \item Factoriser $G$.
        \item Résoudre l'équation $G=0$.
    \end{enumerate}

    \exo{Type Brevet}{Etape8}
    \begin{enumerate}
        \item On pose $H=16x^2-49+(3x-5)(4x+7)$
        \item Factoriser $16x^2-49$ puis $H$.
        \item Résoudre l'équation $H=0$.
    \end{enumerate}
\end{multicols}