
\begin{multicols}{3}
    \exo{Représenter}{Egale1} $$4x+8 \boldsymbol{\neq} -4(-x+2)$$

    \exo{Représenter}{Egale2} $$7x+5 \boldsymbol{=} 7\left(x+\frac{5}{7}\right)$$

    \exo{Représenter}{Egale3} $$3x(2x+1) -2x \boldsymbol{\neq} 6x^2+2x$$

    \exo{Représenter}{Egale4} $$x^2+3x(2x-2) \boldsymbol{=} 7x^2-6x$$ 

    \exo{Représenter}{Egale5} $$8 \boldsymbol{=} x^2-2x(0,5x+1)+2(x+4)$$ 


    \exo{Représenter}{Egale6} $$(2x+1)(3x+4) \boldsymbol{\neq} 6x^2+4+10x$$ 

    \exo{Représenter}{Egale7} $$x^2+3x(2x-2) \boldsymbol{=} 7x^2-6x$$ 

    \exo{Représenter}{Egale8} $$8 -x^2 \boldsymbol{\neq}(4+x)(4-x)$$


    \exo{Représenter}{Egale9} $$(2x-1)(3x+4) \boldsymbol{=} -4+6x^2+5x$$ 

    \exo{Représenter}{Egale10} $$(2x-3)(x+2) \boldsymbol{=} (x-1)(2x+3)-3$$ 

    \exo{Représenter}{Egale11} $$(3x-3)(2x+8) \boldsymbol{=} (x-1)(6x+24)$$


    \exo{Représenter}{Egale12} $$(x-3)(x+2) \boldsymbol{\neq} (x-2)(x+3)$$ 
\end{multicols}